src/sys_verif/notes/ownership.v
@@ -99,8 +99,16 @@ Qed.
 
 (*| The code in this example includes a type annotation on the load, with the type `#uint64T`. This type is required since this load is not a core primitive, but instead a function. Composite values like structs are not stored in one heap location, but laid out with one field per location, and `![#s] #l` with a struct type `s` would load the fields individually. However, this specification hides that complexity: as long as the type `uint64T` matches the type of data in the points-to assertin (`w64`), we get the expected specification for loads. |*)
 
+(*| ## Read-only ownership: fractional permissions {#read-only}
+
+Fractional permissions are an approach to reasoning about read-only access in separation logic.
+
+This concept is explained as part of the Program Proofs guide in [fractional permissions](./program-proofs/fractions.md).
+
+|*)
+
 (*| 
-## Structs
+## Modeling Structs
 
 Ownership over pointers to structs is more interesting than ownership over plain variables.
 
@@ -134,6 +142,11 @@ func ExamplePerson() Person {
 }
 ```
 
+|*)
+
+(*| 
+Goose models the struct as a tuple, but it hides this fact behind a nicer interface to treat the struct as a Rocq record. It generates a Rocq record called `Person.t` to model the data in a Go `Person` struct:
+
 ```rocq
 Module Person.
 Record t := mk {
@@ -144,98 +157,70 @@ Record t := mk {
 End Person.
 ```
 
-The ownership principle for structs can best be described by comparing `Older` and `GetAge`. Notice that `Older` only needs ownership (or permission to access) the field Age, not the entire struct `p *Person`. Similarly, `GetAge` is fundamentally about extracting ownership over the single field `p.Age`; different (but related) assertions are needed to give the ownership of `p` and of `&p.Age`.
+A Rocq Record is essentially an inductive type with one constructor (called `Person.mk` in this case), but this command also generates functions for each field (for example, `Person.FirstName'`) to get one field from a `Person.t` record. Goose relates these Gallina fields to the GooseLang model of field references.
 
-Methods on structs are actually quite easy to model: `Name` becomes a function `Person__Name` that takes `p` as its first argument. The struct name is prepended to disambiguate this function from another function `Name` in the same scope (or another struct method called `Name`). Whenever Go calls a method on a struct, it is translated to a call to the appropriate function. If you're not sure how Go methods work as a language feature, read the [Go tour on methods](https://go.dev/tour/methods/1).
-
-You might wonder if this is too simple. Go's methods are actually what is simple in this case: what complicates methods in object-oriented languages with inheritance like Java or C++ is that a call to a method might actually resolve to a superclass implementation, and in fact the exact method called might be dynamic. Go has `interface`s that behave somewhat similarly, which Goose does not model; interfaces are still simpler than inheritance and with some engineering Goose could support them without too much pain. (Inheritance could also be modeled but with a little more pain.)
-
-Having handled methods, structs introduce two main challenges: how to model struct values, and how to model struct pointers.
-
-Let's start with modeling struct values. The basic strategy is to translate a value of type `p: Person` to a tuple of the fields of the struct. To keep GooseLang simple, it only has binary pairs, not arbitrary-sized tuples, and functions `Fst` and `Snd` access the elements of a pair (these were called $\pi_1$ and $\pi_2$ way back in the `expr` language, but we'll use names for them now). With the tuple model, a person as in the `ExamplePerson()` function above would have the value `(#"Ada", (#"Lovelace", #(W64 25)))`.
-
-To model field access, like `p.FirstName` that shows up in the `Name` method, we need to use `Fst` and `Snd` appropriately based on what index the field has; in this case it's easy and the model should be `Fst p`.
-
-### Exercise: accessing other fields
-
-:::: info Exercise
-
-What's the right model of `p.LastName` and `p.Age`?  Remember that we organized the tuple as `(#"Ada", (#"Lovelace", #(W64 25)))`.
-
-::: details Solution
-
-`p.LastName` should be modeled as `Fst (Snd p)` and `p.Age` is `Snd (Snd p)`.
-
-:::
-
-::::
-
-### Struct pointers
-
-We might be tempted to say a pointer to a struct is a location, and we store the tuple in the heap. The code `p.Older(delta)` above could be translated to something like `p <- (FirstName p, (LastName p, Age p + delta))` - notice that this method takes a struct _pointer_ and not a _value_ in Go, and this is reflected in how we use `p` in the model. This approach to translating structs is basically fine for this case (even if a bit complicated to implement), but it is limited.
+Next, we need to model structs in memory. We might be tempted to say a pointer to a struct is a location, and we store the tuple at that location in the heap. The code `p.Older(delta)` above could be translated to something like `p <- (FirstName p, (LastName p, Age p + delta))` - notice that this method takes a struct _pointer_ and not a _value_ in Go, and this is reflected in how we use `p` in the model.
 
 The third method, `GetAge`, however, would be problematic for this model. What pointer should it return? We know what should happen if we read and write to that pointer, but don't have a value to return for just `GetAge`.
 
-The solution Goose uses is not to use a single location for a struct, but instead _one per field_. The heap locations are all laid out contiguously, just like an array. Thus the model for `GetAge` is actually `GetAge := λ: "ℓ", "ℓ" +ₗ 2`, where 2 is the index of the `Age` field.
+The solution Goose uses is not to store a struct in a single heap cell, but instead _one per field_. The heap locations are all laid out contiguously, just like an array. Thus the model for `GetAge` is actually `GetAge := λ: "ℓ", "ℓ" +ₗ 2`, where 2 is the index of the `Age` field.
 
-## Proofs using structs
-
-Now let's see how this theory translates to Goose. First of all, we don't literally work with field offsets as literals; we would want constants based on the field names for those immediately in the proofs, and the actual translation uses field names in an even better way.
-
-Here's the actual translation of the structs above:
+The translated code for struct operations doesn't directly use offsets but instead uses a helper function `struct.field_ref` to compute the offset from a struct type and field name. We can see this used throughout the model in the translation of the code above:
 
 ```rocq
-Definition Person := struct.decl [
+Definition Person : go_type := structT [
   "FirstName" :: stringT;
   "LastName" :: stringT;
   "Age" :: uint64T
 ].
 
-Definition Person__Name: val :=
-  rec: "Person__Name" "p" :=
-    ((struct.loadF Person "FirstName" "p") +
-    #(str" ")) +
-    (struct.loadF Person "LastName" "p").
+Definition Person__Nameⁱᵐᵖˡ : val :=
+  λ: "p" <>,
+    exception_do (let: "p" := (mem.alloc "p") in
+    return: (((![#stringT] (struct.field_ref #Person #"FirstName"%go "p")) + #" "%go) + (![#stringT] (struct.field_ref #Person #"LastName"%go "p")))).
 
-Definition Person__Older: val :=
-  rec: "Person__Older" "p" "delta" :=
-    struct.storeF Person "Age" "p"
-                  ((struct.loadF Person "Age" "p") + "delta");;
-    #().
+Definition Person__Olderⁱᵐᵖˡ : val :=
+  λ: "p" "delta",
+    exception_do (let: "p" := (mem.alloc "p") in
+    let: "delta" := (mem.alloc "delta") in
+    do:  ((struct.field_ref #Person #"Age"%go (![#ptrT] "p")) <-[#uint64T] ((![#uint64T] (struct.field_ref #Person #"Age"%go (![#ptrT] "p"))) + (![#uint64T] "delta")));;;
+    return: #()).
 
-Definition Person__GetAge: val :=
-  rec: "Person__GetAge" "p" :=
-    struct.fieldRef Person "Age" "p".
+Definition Person__GetAgeⁱᵐᵖˡ : val :=
+  λ: "p" <>,
+    exception_do (let: "p" := (mem.alloc "p") in
+    return: (struct.field_ref #Person #"Age"%go (![#ptrT] "p"))).
 
-Definition ExamplePerson: val :=
-  rec: "ExamplePerson" <> :=
-    struct.mk Person [
-      "FirstName" ::= #(str"Ada");
-      "LastName" ::= #(str"Lovelace");
-      "Age" ::= #25
-    ].
+(* go: struct.go:21:6 *)
+Definition ExamplePersonⁱᵐᵖˡ : val :=
+  λ: <>,
+    exception_do (return: (let: "$FirstName" := #"Ada"%go in
+     let: "$LastName" := #"Lovelace"%go in
+     let: "$Age" := #(W64 25) in
+     struct.make #Person [{
+       "FirstName" ::= "$FirstName";
+       "LastName" ::= "$LastName";
+       "Age" ::= "$Age"
+     }])).
 ```
 
-The first thing to notice is that even the struct `Person` is translated. It doesn't produce a GooseLang expression, but instead a "struct declaration", which records the fields and their types in a list - we'll come back to those types later, which are most important when we have nested structs. This declaration is later used by _Gallina_ functions like `struct.loadF` and `struct.storeF` to figure out what offset the fields have.
+The first thing to notice is that even the struct `Person` is translated. It doesn't produce a GooseLang expression, but instead a `go_type`, which records the fields and their types in a list - we'll come back to those types later, which are most important when we have nested structs. This declaration is later used by the _Gallina_ function `struct.field_ref` to figure out what offset the fields have.
 
-The easiest model to understand is `GetAge`, which is entirely based on the Gallina function `struct.fieldRef`. The implementation searches the `Person` declaration for the field `Age` and returns a GooseLang function that takes the right offset from the input location, 2 in this case.
+The easiest model to understand is `GetAge`, which is entirely based on the function `struct.field_ref`. The implementation searches the `Person` declaration for the field `Age` and returns a GooseLang function that takes the right offset from the input location, 2 in this case. We prove that the GooseLang function `struct.field_ref` computes a Gallina function `struct.field_ref_f` (you'll see that show up in proofs).
 
-Similarly, `struct.mk` takes a struct declaration and a list of field values and assembles them into a struct value, a tuple with all the fields. This is needed since a struct literal in Go need not be in the same order as the declaration (what would go wrong if we assumed it was?) and because fields can be omitted, in which case they get the zero value for their type. The declaration records both the order of the fields and the types for this reason.
+Similarly, `struct.make` takes a struct declaration and a list of field values and assembles them into a struct value, a tuple with all the fields. This is needed since a struct literal in Go need not be in the same order as the declaration (what would go wrong if we assumed it was?) and because fields can be omitted, in which case they get the zero value for their type. The declaration records both the order of the fields and the types for this reason.
 
-The other Gallina functions in this example, `struct.loadF` and `struct.storeF` are very similar to `struct.fieldRef`, except that they also do a store or load at the location.
+## Ownership of structs
 
-Goose has a nice set of reasoning principles for structs, which extend the basic points-to assertion we've been using for heap locations. Let's see what specifications for the code above look like.
+Goose has two key ideas for reasoning about structs: first, the typed points-to assertion allows ownership over structs, not just base data, and second, a points-to with a struct value is actually a separating conjunction of all of its fields.
+
+To see these ideas in action, let's start with a function that doesn't involve ownership:
 
 |*)
 
-(*| Goose does actually model struct values as tuples, and doesn't (yet) have a better way to write them in specs.
-
-In practical use, we typically define a Gallina record and relate these records to the GooseLang representation, and then most specs work with the Gallina record and not with these tuples.
-
-Notice also that there's an extra unit value at the end; this makes the recursive functions for accessing fields much simpler. |*)
 Lemma wp_ExamplePerson :
   {{{ is_pkg_init heap.heap }}}
-    @! heap.heap.ExamplePerson #()
+    @! heap.ExamplePerson #()
   {{{ RET #(heap.Person.mk "Ada" "Lovelace" (W64 25)); True }}}.
 Proof.
   wp_start as "_".
@@ -243,25 +228,9 @@ Proof.
   done.
 Qed.
 
-Lemma wp_Person__Name (firstName lastName: go_string) (age: w64) :
-  {{{ is_pkg_init heap.heap }}}
-  (heap.Person.mk firstName lastName age) @ heap.Person.id @ "Name" #()
-  {{{ RET #(firstName ++ " " ++ lastName)%go; True }}}.
-Proof.
-  wp_start as "#init".
-  wp_alloc p_l as "p". wp_pures.
-  iApply struct_fields_split in "p". iNamed "p".
-  cbn [heap.Person.FirstName' heap.Person.LastName' heap.Person.Age'].
-  wp_auto.
-  iDestruct ("HΦ" with "[]") as "HΦ".
-  { done. }
-  iExactEq "HΦ".
-  f_equal.
-  f_equal.
-  rewrite -app_assoc //.
-Qed.
+(*| `ExamplePerson` returns a struct value. We write the specification using Person.t, and use `#` to turn it into the GooseLang value that is actually returned (which is a tuple, not the Gallina record). |*)
 
-(*| It's helpful to see the struct reasoning where `*Person` gets allocated before seeing how to use it. For that we'll use this function:
+(*| The next example illustrates ownership over a struct pointer. It's helpful to see this in a context where `*Person` initially gets allocated. For that we'll use this function:
 
 ```go
 func ExamplePersonRef() *Person {
@@ -273,11 +242,28 @@ func ExamplePersonRef() *Person {
 }
 ```
 
-The postcondition of the following spec introduces the _struct field points-to_. `l ↦s[heap.Person :: "Age"] (W64 25)` combines calculating an offset from `l` for the Age field of Person (that is, computing `l +ₗ #2`) with asserting that the value at that location is `#25`.
+|*)
+
+(*| This specification shows that the typed points-to can be used for something other than a base literal. The underlying mechanism is the `IntoVal` typeclass, used for both `#` and `l ↦ v`. |*)
+Lemma wp_ExamplePersonRef :
+  {{{ is_pkg_init heap.heap }}}
+    @! heap.ExamplePersonRef #()
+  {{{ (l: loc), RET #l;
+      l ↦ (heap.Person.mk "Ada" "Lovelace" (W64 25)) }}}.
+Proof.
+  wp_start as "_".
+  wp_alloc l as "p".
+  wp_pures.
+  iApply "HΦ".
+  iFrame.
+Qed.
+
+(*| 
+As discussed above, a Person struct in memory is not stored in a single location. The points-to above is actually a separating conjunction over three smaller points-to assertions, one for each field. We can break it down into _struct field points-to_ assertions of the form `l ↦s[heap.Person :: "Age"] (W64 25)`. This is actually notation for a simpler concept: `(struct.field_ref_f heap.Person "Age" l) ↦ (W64 25)`. That is, owning a struct field is simply owning an appropriate offset from the base pointer, computed based on the struct and field name.
 
 |*)
 
-Lemma wp_ExamplePersonRef :
+Lemma wp_ExamplePersonRef_fields :
   {{{ is_pkg_init heap.heap }}}
     @! heap.ExamplePersonRef #()
   {{{ (l: loc), RET #l;
@@ -288,16 +274,34 @@ Lemma wp_ExamplePersonRef :
 Proof.
   wp_start as "#init".
   wp_alloc l as "p".
-  (*| Notice in the goal above how the struct allocation produced a `p ↦[struct.t heap.Person] v` assertion. This is actually the same as the points-to assertion we've been using all along, albeit with a more complex type. This assertion actually says that `v` is a tuple with the right structure to be a `Person` struct, and its three values are laid out in memory starting at `p`.
-
-Now look at what the following line of proof does to the goal.
- |*)
   iApply struct_fields_split in "p". iNamed "p".
   cbn [heap.Person.FirstName' heap.Person.LastName' heap.Person.Age'].
   (*| The theorem `struct_fields_split` gives a way to take any points-to assertion with a struct type and split it into its component field points-to assertions, which is what the postcondition of this spec gives. |*)
   wp_pures.
   iApply "HΦ".
   iFrame.
+Qed.
+
+(*| The two concepts of a single points-to for the whole struct and individual field points-to assertions are the main ideas for how Goose handles ownership of struct. We see them used throughout the rest of the examples above: |*)
+
+Lemma wp_Person__Name (firstName lastName: go_string) (age: w64) :
+  {{{ is_pkg_init heap.heap }}}
+  (heap.Person.mk firstName lastName age) @ heap.Person.id @ "Name" #()
+  {{{ RET #(firstName ++ " " ++ lastName)%go; True }}}.
+Proof.
+  wp_start as "#init".
+(*| Notice how the following `wp_pures` call transforms `struct.field_ref` into `#(struct.field_ref_f ...)` - this is from a Goose-provided theorem that relates the GooseLang code to a Gallina function. |*)
+  wp_alloc p_l as "p". wp_pures.
+  (*| The `struct_fields_split` theorem turns a pointer to a struct into pointers for its individual fields. |*)
+  iApply struct_fields_split in "p"; iNamed "p"; 
+  cbn [heap.Person.FirstName' heap.Person.LastName' heap.Person.Age'].
+  wp_auto.
+  iDestruct ("HΦ" with "[]") as "HΦ".
+  { done. }
+  iExactEq "HΦ".
+  f_equal.
+  f_equal.
+  rewrite -app_assoc //.
 Qed.
 
 Lemma wp_Person__Older (firstName lastName: byte_string) (age: w64) (p: loc) (delta: w64) :
@@ -321,7 +325,7 @@ Proof.
   iFrame.
 Qed.
 
-(*| Here is one spec for `GetAge`, which results in breaking off the age field into its points-to assertion. |*)
+(*| Here is one possible spec for `GetAge`, which results in breaking off the age field into its points-to assertion. Note that this spec allows the caller to retain ownership over the other fields, as opposed to a spec which only gave `age_l ↦ age` in the postcondition. |*)
 Lemma wp_GetAge (firstName lastName: byte_string) (age: w64) (p: loc) (delta: w64) :
   {{{ is_pkg_init heap.heap ∗
       "first" :: p ↦s[heap.Person :: "FirstName"] firstName ∗
@@ -337,7 +341,6 @@ Lemma wp_GetAge (firstName lastName: byte_string) (age: w64) (p: loc) (delta: w6
 Proof.
   wp_start as "H". iNamed "H".
   wp_auto.
-  (* this works pleasantly well, even with complicated struct references *)
   iApply "HΦ".
   iFrame.
 Qed.
@@ -350,15 +353,15 @@ Go has a slice type `[]T`, a generic type that works for any element type `T`.
 
 Slices in Go are implemented as a struct value with a pointer, a length, and a capacity; this is also how they are modeled in GooseLang. It is helpful to know this implementation detail to understand how they work, and it is also a common pattern for dynamically sized arrays (e.g., C++'s `std::vector` and Rust's `Vec` are almost identical).
 
-You can read more about Rust slices in this post on [Go data structures](https://research.swtch.com/godata) or in even more detail in this [post on slices and append](https://go.dev/blog/slices). Below are some basic details.
+You can read more about Go slices in this post on [Go data structures](https://research.swtch.com/godata) or in even more detail in this [post on slices and append](https://go.dev/blog/slices). Below are some basic details.
 
 More primitive than slices are arrays. An array is a contiguous block of memory, and we interact with them through a pointer to the first element. A slice is a "view" into a piece of an array (possibly the entire thing, but not necessarily). You can think of a slice as containing (at any given time) a sequence of elements. The slice is a (pointer, length, capacity) tuple, where the pointer points to the first element in the slice and the length says how many elements are in the slice. The array in memory is contiguous, so we can find any element by taking an offset from the pointer. Finally, the capacity tracks elements past the length that are allocated and in the array, which is memory available to grow the slice if elements are appended.
 
-In Go, the common idiom for appending to a slice `s []T` is `s = append(s, x)`. This is because if `s` has no spare capacity, `append` allocates a new, larger array and copies the elements over to it; this cannot change `s` since this is passed by value, so instead the new slice is returned. When a slice is grown, typically its capacity will be double the original length, to amortize the cost of copying over the elements; hopefully you saw something like this in a data structure class, perhaps as the first example of an amortized analysis.
+The Go `append(s, x)` operation appends to a slice and returns a new slice. If `s` has spare capacity, the new element is stored there and the new slice has the same pointer as the old one, but with its length increased by 1. On the other hand if `s` has no spare capacity, `append` allocates a new, larger array and copies the elements pointed to by `s` over to it. When a slice is grown, typically its capacity will be double the original length, to amortize the cost of copying over the elements; hopefully you saw something like this in a data structure class (it's often the first example shown of amortized cost analysis). A common idiom for appending to a slice `s []T` is `s = append(s, x)`, since we typically want to only use the new slice.
 
 ### Reasoning about slices
 
-The basic assertion for working with slices is `own_slice s t dq xs`. `s` is a `Slice.t`, a Coq record representing the slice value (the triple of pointer, length, and capacity); in GooseLang code, you will instead use `slice_val s : val`. `t` is the type of elements, similar to the types used for structs and struct fields. `dq` is a fraction, explained below; for now we will pretend like it's always `DfracOwn 1`. Finally, `xs` is a Gallina `list` of the elements of the slice. The overall result is an assertion that gives ownership over the slice `s`, and records that it has the elements `xs`.
+The basic assertion for working with slices is `own_slice t dq xs`. `s` is a `Slice.t`, a Rocq record representing the slice value (the triple of pointer, length, and capacity); GooseLang code will use `#s`, the standard way of converting Gallina values to GooseLang values. `dq` is a fraction, explained below; for now we will pretend like it's always `DfracOwn 1`. Finally, `xs` is a Gallina `list V` of the elements of the slice, with the same flexibility for the type `V` as used in points-to assertions, namely `V` can be any type that satisfies `IntoVal V`. The overall result is an assertion that gives ownership over the memory referenced by the slice `s`, and records that it has the elements `xs`.
 
 This abstraction uses typeclasses so the type of `xs` can vary, so for example we can use `list w64` for a slice of integers. You can see this in the type signature for `own_slice`, where there are parameters `V: Type` and `IntoVal V`:
 |*)
@@ -375,27 +378,78 @@ You can ignore this whole string of parameters, which are related to Goose suppo
   → ∀ {ext_ty : ext_types ext}
 ```
 
-Getting and setting slice elements have reasonable specifications:
-
-TODO: fix the written explanation in this lecture: slice operations are now based on getting a reference and using it, not `SliceGet` and `SliceSet`
+GooseLang models loading and storing slice elements in a similar way to struct field operations: a GooseLang function `slice.elem_ref` computes a pointer to the relevant element (the analogous Gallina function is `slice.elem_ref_f`), and then that element pointer can be used like any other pointer. We can see that in these two specifications:
 
 |*)
 
 Check wp_load_slice_elem.
 
-(*| We got this specification using `Check` rather than copying it from the Perennial source code. Notice that the Hoare triple notation is not used here (I'm not entirely sure why, possibly a bug in the notations). You should still be able to read this specification, if you understood the "continuation-passing style" encoding of Hoare triple used in Iris.
+(*| We got this specification using `Check` rather than copying it from the Perennial source code.
 
-The one complication with this particular specification is that its precondition requires the caller to pass the value `v0` that is in the slice. `SliceGet` itself requires `i` to be in-bounds (otherwise `s[i]` panics in Go), and `vs !! uint.nat i = Some v0` has the side of enforcing this obligation, and the postcondition then uses the same value `v0`.
+One complication in using this specification is that its precondition requires the caller to pass the value `v0` that is in the slice. This automatically enforces that the index is less than the length of the slice, that is, `sint.nat i < length vs` (we separately need the index to be non-negative, hence the precondition `0 ≤ sint.Z i`).
+
+Storing is fairly similar:
 |*)
 
-(*| Storing into a slice requires a proof `is_Some (vs !! uint.nat i)`, which similarly guarantees that `i` is in-bounds, but the original value is not needed. The postcondition uses `<[uint.nat i := v]> vs` which is a Gallina implementation of updating one index of a list (it's notation for the function `insert` from std++).
+Check wp_store_slice_elem.
 
-You may notice that there's an arbitrary `q : dfrac` in the specification for `SliceGet`, while `SliceSet` has `DfracOwn 1`. This difference is no accident and corresponds to the fact that `SliceGet` works even on a _read-only_ slice while `SliceSet` needs to be able to modify the input slice. We'll cover the mechanism with fractions [later on](#read-only).
+(*| This slightly complicated proof illustrates both the load and store specs above as well as how to do the arithmetic reasoning required.
+
+The code being verified is a one-liner:
+
+```go
+func SliceSwap(s []int, i, j int) {
+	s[i], s[j] = s[j], s[i]
+}
+```
+
+|*)
+Lemma wp_SliceSwap (s: slice.t) (xs: list w64) (i j: w64) (x_i x_j: w64) :
+  {{{ is_pkg_init heap.heap ∗ s ↦* xs ∗ ⌜xs !! sint.nat i = Some x_i ∧ xs !! sint.nat j = Some x_j⌝ ∗ ⌜0 ≤ sint.Z i ∧ 0 ≤ sint.Z j⌝ }}}
+    @! heap.SliceSwap #s #i #j
+  {{{ RET #(); s ↦* <[ sint.nat j := x_i ]> (<[ sint.nat i := x_j ]> xs) }}}.
+Proof.
+  wp_start as "(Hs & [%Hi %Hj] & %Hbound)".
+  wp_auto.
+
+  (* The slice specs require a bit of boilerplate to prove all the in-bounds requirements. *)
+  pose proof Hi as Hi_bound.
+  apply lookup_lt_Some in Hi_bound.
+  pose proof Hj as Hj_bound.
+  apply lookup_lt_Some in Hj_bound.
+
+  iDestruct (own_slice_len with "Hs") as %Hlen.
+  (* slice.elem_ref requires calling [wp_pure] and then proving that the indices are in-bounds, since Go panics even if you just compute these indices *)
+  wp_pure.
+  { word. }
+  wp_apply (wp_load_slice_elem with "[$Hs]") as "Hs".
+  { word. }
+  { eauto. }
+
+  wp_pure; first word.
+  wp_apply (wp_load_slice_elem with "[$Hs]") as "Hs"; first word.
+  { eauto. }
+
+  wp_pure; first word.
+  wp_apply (wp_store_slice_elem with "[$Hs]") as "Hs"; first word.
+
+  wp_pure; first word.
+  wp_apply (wp_store_slice_elem with "[$Hs]") as "Hs".
+  { autorewrite with len. word. }
+  iApply "HΦ".
+  iFrame.
+Qed.
+
+(*| Storing into a slice requires only a proof that the index is in-bounds. The postcondition uses `<[sint.nat i := v]> vs` which is a Gallina implementation of updating one index of a list (it's notation for the function `insert` from std++).
+
+You may notice that there's an arbitrary `q : dfrac` in the specification for `wp_load_slice_elem`, while `wp_store_slice_elem` does not have a fraction (it is implicitly 1). This is analogous to the read-only ownership for plain pointers that we saw earlier.
 |*)
 
 (*| ### Appending to a slice
 
-The capacity of a slice is interesting in the model because it turns out ownership of the capacity is separate from ownership of the elements. Consider the following code, which splits a slice:
+The ownership reasoning for appending to a slice turns out to be especially interesting in Go. The way this shows up is that it turns out that owning the logical _elements_ of a slice (the memory for `s.(slice.len_f)` elements, starting from the base pointer of the slice) is separate from the ownership of the _capacity_ (the memory from the length up to the capacity).
+
+Consider the following code, which splits a slice:
 
 ```go
 s := []int{1,2,3}
@@ -403,7 +457,7 @@ s1 := s[:1]
 s2 := s[1:]
 ```
 
-What is not obvious in this example is that `s1` has a capacity that _overlaps_ with that of `s2`. Specifically, the behavior of this code is surprising (you can [run it yourself](https://go.dev/play/p/yhcjYdVBVjo) on the Go playground):
+What is not obvious in this example is that in Go, `s1` has a capacity that _overlaps_ with that of `s2`. Specifically, the behavior of this code is surprising (you can [run it yourself](https://go.dev/play/p/yhcjYdVBVjo) on the Go playground):
 
 ```go
 s := []int{1,2,3}
@@ -418,119 +472,51 @@ Goose accurately models this situation. If `s = (ptr, l, c)`, we know from const
 
 In proofs, Goose separates out the predicates for ownership of a slice's elements (between 0 and its length) and its capacity (from length to capacity).
 
-- `own_slice_small s dq t xs` asserts ownership only over the elements within the length of `s`, and says they have values `xs`.
-- `own_slice_cap s t` asserts ownership over just the capacity of `s`, saying nothing about their contents (but they must have type `t`).
-- `own_slice s dq t xs := own_slice_small s dq t xs ∗ own_slice_cap s t` asserts ownership over the elements and capacity.
+- `own_slice s dq xs` asserts ownership only over the elements within the length of `s`, and says they have values `(xs: list V)`.
+- `own_slice_cap V s dq` asserts ownership over just the capacity of `s`, saying nothing about their contents. It takes the Gallina type of elements `V`. This ownership may be fractional, though it is typically 1.
+- `own_slice s dq xs ∗ own_slice_cap V s (DfracOwn 1)` asserts ownership over the elements and capacity of slice `s`.
 
 These predicates are just definitions that are separating conjunctions over regular points-to facts for the elements. In the context of the example above, with `s = (ptr, 3, 4)` (notice we picked a capacity of 4), these predicates are equal to the following:
 
-- `own_slice_small s [1;2;3] = (ptr + 0) ↦ 1 ∗ (ptr + 1) ↦ 2 ∗ (ptr + 2) ↦ 3`
+- `own_slice s [1;2;3] = (ptr + 0) ↦ 1 ∗ (ptr + 1) ↦ 2 ∗ (ptr + 2) ↦ 3`
 - `own_slice_cap s [1;2;3] = ∃ x, (ptr + 3) ↦ x`
 - ```
-  own_slice_small (s[1:]) [2; 3]
+  own_slice (s[1:]) [2; 3]
    = ((ptr + 1) + 0) ↦ 2 ∗ ((ptr + 1) + 1) ↦ 3
    = (ptr + 1) ↦ 2 ∗ (ptr + 2) ↦ 3
   ```
 
-Confirm for yourself that `own_slice_small` and `own_slice_cap` are disjoint; without that, `own_slice` wouldn't be useful since it would be equivalent to $\False$.
+Confirm for yourself that `own_slice` and `own_slice_cap` are disjoint; without that, we could never own both the slice and capacity.
 
 The main specification related to capacity is the one for append:
 
 ```rocq
-Lemma wp_SliceAppend s t vs x :
-  {{{ own_slice s t (DfracOwn 1) vs ∗ ⌜val_ty x t⌝ }}}
-    SliceAppend t s x
-  {{{ s', RET slice_val s'; own_slice s' t (DfracOwn 1) (vs ++ [x]) }}}.
+Lemma wp_slice_append (s: slice.t) (vs: list V) (s2: slice.t) (vs': list V) dq :
+  {{{ s ↦* vs ∗ own_slice_cap V s (DfracOwn 1) ∗ s2 ↦*{dq} vs' }}}
+    slice.append #t #s #s2
+  {{{ (s': slice.t), RET #s';
+      s' ↦* (vs ++ vs') ∗ own_slice_cap V s' (DfracOwn 1) ∗ s2 ↦*{dq} vs' }}}.
 ```
 
-Notice that `own_slice` appears in the pre- and post-condition; it would be unsound to use `own_slice_small` here, since appending modifies the capacity of a slice.
+Notice that `own_slice_cap` appears in the pre-condition, with fraction 1; this is required since append will write to the elements in the capacity if there is room.
 
-What is key to understanding the Go example above is that the Go expression `s[:n]` is ambiguous as to how it handles ownership. The capacity of `s[:n]` and `s[n:]` overlap; if we model `s[:n]` with `slice_take s n` and `s[n:]` as `slice_drop s n`, then there are two main choices for how to divide ownership when taking a prefix:
+With this specification, we can now return to the example above. What is key to understanding the Go example above is that the Go expression `s[:n]` is ambiguous as to how it handles ownership. The capacity of `s[:n]` and `s[n:]` overlap; if we model `s[:n]` with `slice.slice_f s 0 n` and `s[n:]` as `slice.slice_f s n s.(slice.len_f)`, then there are two main choices for how to divide ownership when taking a prefix (taking some liberty to omit fractions and use n as both a w64 and a nat)
 
-- `own_slice s dq t xs ⊢ own_slice (slice_take s dq t (take xs n))`. Drop any ownership over the elements after `n`, but retain the capacity of the smaller slice.
-- `own_slice_small s dq t xs ⊢ own_slice_small (slice_take s dq t (take xs n)) ∗ own_slice_small (slice_drop s dq t (drop xs n))`. Split ownership, but lose the ability to append to the prefix.
+- `own_slice s xs ∗ own_slice_cap s V ⊢ own_slice (slice.slice_f s 0 n) (take xs n))`. Drop any ownership over the elements after `n`, but retain the capacity of the smaller slice.
+- `own_slice s xs ⊢ own_slice (slice.slice_f s 0 n) (take xs n)) ∗ own_slice (slice.slice_f s n s.(slice.len_f) (drop xs n))`. Split ownership, but lose the ability to append to the prefix.
 
 There is one more possibility which is a slight variation on splitting:
-- `own_slice s dq t xs ⊢ own_slice_small (slice_take s dq t (take xs n)) ∗ own_slice (slice_drop s dq t (drop xs n))`. If we start out with ownership of the capacity, we can split ownership and still be able to append to the _second_ part (its capacity is the capacity of the original slice). We can actually derive this from the lower-level fact that `slice_cap s t ⊣⊢ slice_cap (slice_skip s n)` if `n` is in-bounds.
+- `own_slice s xs ∗ own_slice_cap s V ⊢ own_slice (slice.slice_f s 0 n) (take xs n)) ∗ own_slice (slice.slice_f s n s.(slice.len_f)) (drop xs n)) ∗ own_slice_cap (slice.slice_f s n s.(slice.len_f))`. If we start out with ownership of the capacity, we can split ownership and still be able to append to the _second_ part (its capacity is the capacity of the original slice). We can actually derive this from the lower-level fact that `slice_cap s V ⊣⊢ slice_cap (slice.slice_f s n s.(slice.len_f)) V` if `n` is in-bounds.
 
 ### Exercise: find the theorems above in Perennial
 
 Either using `Search` or by looking at the source code in Perennial, find the theorems above.
 
-The relevant source code is the file `src/goose_lang/lib/slice/typed_slice.v` in Perennial (you can use the submodule copy in your exercises repo).
+The relevant source code is the file `new/golang/theory/slice.v` in Perennial (you can use the submodule copy in your exercises repo).
 
 ### Exercise: attempt a proof outline for the append example
 
 Try to use the predicates and rules for slice ownership to give a proof outline for the append example. At some point you will get stuck, because the reasoning principles don't give a way to verify the code above - this is fine in that we don't really intend to verify odd code like the above, but seeing exactly where you get stuck is instructive for learning how the rules work.
-
-|*)
-
-(*| ## Read-only ownership: fractional permissions {#read-only}
-
-Fractional permissions are an approach to reasoning about read-only access in separation logic.
-
-This concept is explained as part of the Program Proofs guide in [fractional permissions](./program-proofs/fractions.md).
-
-|*)
-
-(*| ### Ownership in iterators
-
-As another example, consider a hashmap with an iteration API that looks like this:
-
-```go
-func PrintKeys(m HashMap) {
-  it := m.KeyIterator()
-  for k, ok := it.Next(); ok {
-      fmt.Println(k)
-  }
-}
-```
-
-That is, we have an API like this (where `Key` is a placeholder for the key type):
-
-```go
-// normal operations:
-func (m HashMap) Get(k Key) (v Value, ok bool)
-func (m HashMap) Put(k Key, v Value)
-func (m HashMap) Delete(k Key)
-
-// iteration:
-func (m HashMap) KeyIterator() *Iterator
-func (it *Iterator) Next() (k Key, ok bool)
-```
-
-Given this API, is this safe?
-
-```go
-// does this work?
-
-func PrintValues(m HashMap) {
-  it := m.KeyIterator()
-  for k, ok := it.Next(); ok {
-      v, _ := m.Get(k)
-      fmt.Println(v)
-  }
-}
-```
-
-What about this one?
-
-```go
-// does this work?
-
-func ClearMap(m HashMap) {
-  it := m.KeyIterator()
-  for k, ok := it.Next(); ok {
-      m.Delete(k)
-  }
-}
-```
-
-::: details Solution
-
-You can't tell from just the API (which does not even describe ownership in comments). For most hashmap implementations, the iterator should be considered to _own_ read-only permission on the entire hashmap. This means that `PrintValues` is safe, but `ClearMap` is not. This problem is often called _iterator invalidation_ since the call to `m.Delete(k)` is considered to _invalidate_ `it` in the next iteration.
-
-:::
 
 |*)
 
